{-# OPTIONS --without-K --rewriting #-}
open import lib.Base
open import lib.Equivalence
open import lib.Equivalence2
open import lib.Univalence
open import lib.Funext
open import lib.NType
open import lib.NType2
open import lib.Funext
open import lib.types.Pi
open import lib.PathGroupoid
open import Magma-basics
open import Group-basics
open import Goal1_isom_groups_are_equal

{- In this file we work towards the second goal of the project: definable subgroups are normal in
   HoTT
-}

module Goal2_definable_subgr_normal {α : ULevel} where


{- In this module, we will prove that the idtoiso function from the goal 1 file is actually
   equivalent to the idtoiso' function defined below. In particular, we need the fact that
   idtoiso idp == idtoiso idp' -}
module _ where

  idtoiso' : {G H : Group {α}} → (G == H) → (G ≃ᴳ H)
  idtoiso' {G} {.G} idp = →ᴳ-id , is-eq (λ z → z) (λ z → z) (λ a → idp) (λ a → idp)

  {- Lemma about props we need later on -}
  paths-are-props : {ℓ : ULevel} {X : Set ℓ} {a b : X} → (isSet : is-set X) → is-prop (a == b)
  paths-are-props {ℓ} {X} {a} {b} isSet = has-level-apply isSet a b

  {- We need a convenient way to show that two isomorphisms are equal. For this, we first
     characterize when two homomorphisms are equal. We prove that a homomorphism is completely
     determined by its map. Secondly, we use this to prove that two isomorphisms are equal when the
     underlying map of the homomorphism is equal
  -}
  module _ {α : ULevel} {G H : Group {α}} where

    {- We give an alternative definition of a group homomorphism -}
    GroupHom' : {α β : ULevel} (G : Group {α}) (H : Group {β}) → Set (lmax α β)
    GroupHom' G H =
      Σ (Group.U G → Group.U H)
        (λ f → ((g₁ g₂ : Group.U G) → f (Group.comp G g₁ g₂) == Group.comp H (f g₁) (f g₂)))

    {- We prove that the two definitions are equivalent -}
    GroupHom-equiv-GroupHom' : GroupHom G H ≃ GroupHom' G H
    GroupHom-equiv-GroupHom' = ((λ hom → (GroupHom.f hom) , (GroupHom.pres-comp hom)) ,
                               record { g =  (λ hom' → group-hom (fst hom') (snd hom'))
                                      ; f-g = λ b → idp ; g-f = λ a → idp ; adj = λ a → idp })

    {- For two homomorphisms of type GroupHom', if their underlying map is equal, than the
       homomorphisms are equal.
    -}
    map-determ-hom' : {hom1 hom2 : GroupHom' G H} → (fst hom1 == fst hom2) → (hom1 == hom2)
    map-determ-hom' {hom1} {hom2} idp =
      pair= idp (λ= (λ g₁ → λ= λ g₂ → prop-path (paths-are-props (Group.set H))
                                                (snd hom1 g₁ g₂) (snd hom2 g₁ g₂)))

    {- Map determines homomorphism for type GroupHom -}
    map-determ-hom : {hom1 hom2 : GroupHom G H} → (GroupHom.f hom1 == GroupHom.f hom2)
                   → (hom1 == hom2)
    map-determ-hom {hom1} {hom2} idp = path
      where
        open is-equiv (Σ.snd GroupHom-equiv-GroupHom')

        f : (GroupHom G H → GroupHom' G H )
        f = Σ.fst GroupHom-equiv-GroupHom'

        path : (hom1 == hom2)
        path =
          hom1 =⟨ ! (g-f hom1) ⟩
          g(f(hom1)) =⟨ ap g (map-determ-hom' idp) ⟩
          g(f(hom2)) =⟨ g-f hom2 ⟩
          hom2 =∎

  {- Now, using the fact that equivalences are propositions we can prove that two isomorphisms are
     equal whenever their homomorphisms is equal. -}
  iso-equiv2 : {G H : Group {α}} → {iso₁ iso₂ : G ≃ᴳ H} → (p : Σ.fst iso₁ == Σ.fst iso₂)
             → iso₁ == iso₂
  iso-equiv2 {G} {H} {.(fst iso₂) , snd} {iso₂} idp =
    pair= idp (prop-path is-equiv-is-prop snd (Σ.snd iso₂))

  {- This again implies that isomorphisms are equal if the underlying map of their homomorphism is
     equal
  -}
  iso-equiv : {G H : Group {α}} → {iso₁ iso₂ : G ≃ᴳ H}
            → (p : GroupHom.f (Σ.fst iso₁) == GroupHom.f (Σ.fst iso₂)) → iso₁ == iso₂
  iso-equiv p = iso-equiv2 (map-determ-hom p)

  {- We can use the fact proven in the goal 1 file that idtoiso when given the identity path
     returns an isomorphism of which the underlying map is the identity map. Since this
     characterizes the whole isomorphism, we can now easilty show that idtoiso idp == idtoiso' idp
  -}
  idtoiso-idp-equiv : {G : Group {α}} →  idtoiso idp == idtoiso' idp
  idtoiso-idp-equiv {G} = iso-equiv (idtoiso-idp-gives-id-map {α} {G})

  {- Finally, we can now use this to prove that idtoiso == idtoiso' -}
  idtoiso-equiv : {G H : Group {α}} → idtoiso {α} {G} {H} == idtoiso' {G} {H}
  idtoiso-equiv {G} {H} = λ= (λ a → lemma a)
    where
      lemma : (a : G == H) → idtoiso a == idtoiso' a
      lemma idp = idtoiso-idp-equiv



{- In this module, we define a function that given an isomorphism between G and H and a subgroup
   of type G, transforms it into a subgroup of type H -}
module _ {G : Group} {H : Group} where

  {- Using a homomorphism from H to G, we can transform any subgroup of G into a subgroup of H -}
  lift-hom-over-subgrp : (hom : H →ᴳ G) → (Subgrp G → Subgrp  H)
  lift-hom-over-subgrp hom sub-g = record { prop = prop-lemma ; f = λ {a} → f-lemma a
                                          ; id = id-lemma ; comp =  λ {a} {b} → comp-lemma a b
                                          ; inv = λ {a} → inv-lemma a}
    where
      open Subgrp sub-g
      open GroupHom hom renaming (f to h-to-g)

      {- We essentially define the new prop to be the prop of sub-g, but then composed with the
         homomorphism from h to g first -}
      prop-lemma : Group.U H → Set α
      prop-lemma h = prop (h-to-g h)

      f-lemma :  (a : Group.U H) → is-prop (prop-lemma a)
      f-lemma a = f

      {- We then use the preserving properties of a homomorphism to show that this map is still
         a subgroup -}
      id-lemma : prop-lemma (Group.e H)
      id-lemma = coe (ap prop (! id-to-id)) id

      comp-lemma : (a b : Group.U H) → prop-lemma a → prop-lemma b → prop-lemma (Group.comp H a b)
      comp-lemma a b prop-a prop-b = coe (ap prop (! (pres-comp a b))) (comp prop-a prop-b)

      inv-lemma : (a : Group.U H) → prop (h-to-g a) → prop (h-to-g (Group.i H a))
      inv-lemma a prop-a = coe (ap prop (! (pres-i a))) (inv prop-a)

  {- With an isomorphism, we just extract the the homomorphism from H to G to create a map
     that transforms any subgroup of G into a subgroup of H -}
  lift-iso-over-subgrp : (iso : G ≃ᴳ H) → (Subgrp G → Subgrp  H)
  lift-iso-over-subgrp iso sub-g = lift-hom-over-subgrp hom sub-g
    where
      hom : H →ᴳ G
      hom = _≃ᴳ_.g-hom iso

{- General lemma proving that function equality proves that the functions are also equal
   on every input. This will be needed in different other proofs -}
funqeq : {β : ULevel} {A B : Set β} {f g : A → B} (p : f == g) (a : A) → (f a == g a)
funqeq idp a = idp


{- We will show in this module that to prove equality between Subgrp's it is sufficient to just
   prove that there is a path between the two prop's. We will need this later on to show that
   two Subgrp's are equal -}
module _ where

  private
    {- First, we give an alternative definition of a subgroup. This definition consists of a Σ-type
       with as first argument the prop function and second argument a proof that this prop is indeed
       a subgroup -}
    record is-subgrp {G : Group {α}} (prop : (Group.U G) → Set α) : Set (lsucc α) where
      private
        module G = Group G
      field
        f : ∀ (a : G.U) → is-prop( prop a)
        id : prop G.e
        comp : ∀ (a b : G.U) → prop a → prop b → prop (G.comp a b)
        inv : ∀ (a : G.U) → prop a → prop (G.i a)

    subgrp' : {G : Group {α}} → Set (lsucc α)
    subgrp' {G} = Σ (Group.U G → Set α) (λ y → is-subgrp {G} y)

    {- We show that any two is-subgrp proofs of the same prop function must be equal. To show this,
       we make use of the fact that is-prop holds for any prop -}
    any-isg-with-same-prop-are-equal : {G : Group {α}} {pr : (Group.U G) → Set α}
                                       (isg1 isg2 : is-subgrp {G} pr) → (isg1 == isg2)
    any-isg-with-same-prop-are-equal {G} isg1 isg2 = =lemma isg1 isg2 f-eq id-eq comp-eq inv-eq
      where
        open is-subgrp
        f-eq : f isg1 == f isg2
        f-eq = λ= (λ a → prop-path has-level-is-prop (f isg1 a) (f isg2 a))

        id-eq : id isg1 == id isg2
        id-eq = prop-path (f isg1 (Group.e G)) (id isg1) (id isg2)

        comp-eq : comp isg1 == comp isg2
        comp-eq = λ= (λ a → λ= (λ b → λ= (λ x → λ= λ y →
          prop-path (f isg1 (Group.comp G a b)) (comp isg1 a b x y) (comp isg2 a b x y))))

        inv-eq : inv isg1 == inv isg2
        inv-eq = λ= (λ a → λ= (λ b →
          prop-path (f isg1 (Group.i G a)) (inv isg1 a b) (inv isg2 a b)))

        =lemma : {G : Group {α}} {pr : (Group.U G) → Set α} (isg1 isg2 : is-subgrp {G} pr)
                 (eq1 : f isg1 == f isg2) (eq2 : id isg1 == id isg2) (eq3 : comp isg1 == comp isg2)
                 (eq4 : inv isg1 == inv isg2) → (isg1 == isg2)
        =lemma record { f = .(f isg2) ; id = .(id isg2) ; comp = .(comp isg2) ; inv = .(inv isg2) }
               isg2 idp idp idp idp = idp

    {- Now we can prove using the lemma above that if there is a path between the prop's, there also
       is a path between the transported version of the accompanying is-subgrp proofs -}
    path-prop-implies-path-isg : {G : Group {α}} (pr1 pr2 : (Group.U G) → Set α) (p : pr1 == pr2)
                                 (subgr1 : is-subgrp {G} pr1) (subgr2 : is-subgrp {G} pr2)
                               → (transport is-subgrp p subgr1 == subgr2)
    path-prop-implies-path-isg pr1 pr2 p subgr1 subgr2 =
      any-isg-with-same-prop-are-equal (transport is-subgrp p subgr1) subgr2

    {- Using the above, it now becomes easy to show that if the prop's of a subgrp' are equal, then
       the whole subgrp's must be equal -}
    subgrp'-eq : {G : Group {α}} (a b : subgrp' {G}) (p : Σ.fst a == Σ.fst b) → (a == b)
    subgrp'-eq a b p =
        subgrp'= a b p (path-prop-implies-path-isg (Σ.fst a) (Σ.fst b) p (Σ.snd a) (Σ.snd b))
      where
        subgrp'= : {G : Group {α}} (a b : subgrp' {G}) (p : Σ.fst a == Σ.fst b)
                   (pt : (transport is-subgrp p (Σ.snd a)) == (Σ.snd b)) → (a == b)
        subgrp'= (fst₁ , snd₁) (.fst₁ , .snd₁) idp idp = idp

    {- Finally, we need to convert the subgrp'eq proof into a proof about Subgrp, so we will show
       that both definitions are equivalent-}
    subgrp-subgrp'-equiv : (G : Group {α}) → Subgrp G ≃ subgrp' {G}
    subgrp-subgrp'-equiv G = f , (record { g = g ; f-g = f-g ; g-f = g-f ; adj = λ a → idp })
      where
        f : Subgrp G → subgrp' {G}
        f record { prop = prop ; f = f ; id = id ; comp = comp ; inv = inv } = prop ,
          record {f = λ a → f {a} ; id = id; comp = λ a b → comp {a} {b}; inv = λ a → inv {a}}

        g : subgrp' {G} → Subgrp G
        g (prop , record { f = f ; id = id ; comp = comp ; inv = inv }) =
          record{ prop = prop ; f = λ {a} → f a ; id = id ; comp = λ {a} {b} → comp a b
                ; inv = λ {a} → inv a}

        f-g : (b : subgrp') → f (g b) == b
        f-g b = idp

        g-f : (a : Subgrp G) → g (f a) == a
        g-f a = idp

  {- Now, using this equivalence and subgrp'-eq holds, we can finally show that if the prop's
     of a Subgrp are equal, then both Subgrp's are equal -}
  subgrp-eq : {G : Group {α}} {a b : Subgrp G} (p : Subgrp.prop a == Subgrp.prop b) → (a == b)
  subgrp-eq {G} {a} {b} p = path
    where
      open is-equiv (Σ.snd (subgrp-subgrp'-equiv G))
      f : Subgrp G → subgrp' {G}
      f = Σ.fst (subgrp-subgrp'-equiv G)

      prf : ((f a) == (f b))
      prf = subgrp'-eq (f a) (f b) p

      path : (a == b)
      path =
        a  =⟨ ! (g-f a) ⟩
        g(f(a)) =⟨ ap g prf ⟩
        g(f(b)) =⟨ g-f b ⟩
        b =∎



{- We show in this module that if you have a map f from groups to subgroups, a particular
   group G and any automorphism between G, then there is a path between the subgroup (f G)
   and the subgroup obtained by applying that automorphism to (f G) -}
module _  (f : (G : Group {α}) → (Subgrp G)) where

  private
    {- We need the fact proven in the goal 1 file that idtoiso(isotoid iso) == iso -}
    iso-id-equiv : {G H : Group {α}} (iso : G ≃ᴳ H) → (idtoiso (isotoid iso)) == iso
    iso-id-equiv {G} {H} iso = is-equiv.g-f (snd (iso≃id {α} {G} {H})) iso

    {- We furthermore need apd as a lemma -}
    apd2 : {l k : ULevel} {X : Set l} {Y : X → Set k} {x x' : X} (f : (x : X) → Y x) (p : x == x')
         → (transport Y p (f x) ) == f x'
    apd2 f idp = idp

    {- We first prove that if we have a path from G to H that the lift-iso-over-subgrp function
       essentially does the same as just transporting it. We use here that idtoiso is equivalent to
       our easier idtoiso', which is definitionally equal to transporting the path -}
    lift-aut-lemma1 : {G H : Group} (p : G == H)
                    → (lift-iso-over-subgrp (idtoiso p)) == (transport Subgrp  p)
    lift-aut-lemma1 {G} {H} idp =
      lift-iso-over-subgrp (idtoiso idp) =⟨ ap lift-iso-over-subgrp idtoiso-idp-equiv ⟩
      lift-iso-over-subgrp (idtoiso' idp) =⟨ λ= (λ g → subgrp-eq idp) ⟩
      transport Subgrp idp =∎

    {- Now we make use of the iso-id-equiv to show that the same holds if we now have an
       automorphism instead of a path. -}
    lift-aut-lemma2 : {G : Group} (aut : G ≃ᴳ G)
                    → lift-iso-over-subgrp aut == transport Subgrp (isotoid aut)
    lift-aut-lemma2 {G} aut =
        lift-iso-over-subgrp aut =⟨ ap lift-iso-over-subgrp (! (iso-id-equiv {G} {G} aut)) ⟩
        lift-iso-over-subgrp (idtoiso (isotoid aut)) =⟨ lift-aut-lemma1 ((isotoid aut)) ⟩
        transport Subgrp (isotoid aut) =∎

  {- Lastly, we combine everything in this statement, where we make use of apd to show that applying
     an automorphism to (f G) is equal to just (f G) -}
  lift-aut-retains-subgrp : {G : Group} (aut : G ≃ᴳ G) → ((lift-iso-over-subgrp aut (f G)) == f G)
  lift-aut-retains-subgrp {G} aut =  funqeq (lift-aut-lemma2 aut) (f G) ∙ (apd2 f (isotoid aut))

{- The statement lift-aut-retains-subgrp is sufficient to show that (f G) is normal, since an
   alternative definition of a normal subgroup is that the subgroup is closed under inner
   automorphisms (conj-aut) and lift-aut-retains-subgrp proves that (f G) is closed under
   any automorphism.

   To derive the result that (f G) is normal as a corollary, we first need to define this
   inner automorphism and prove that it is indeed an automorphism -}
module ConjAut {G : Group {α}} where

  private

    open Group G
    {- Here we define the conjugation map -}
    conj-map : (a : U) → (U → U)
    conj-map a g = a · (g · (i a))

    {- This is a lemma about how the conjugation map behaves that will be useful for
       proving that the conj-map is an automorphism -}
    conj-map-inv : (a : U) → (conj-map a) ∘ (conj-map (i a)) == idf U
    conj-map-inv a = λ= (λ x →
      (conj-map a (conj-map (i a) x)) =⟨ idp ⟩
      a · (( (i a) · (x · (i (i a))) ) · (i a))
        =⟨ ! (associative a ((i a) · (x · (i (i a)))) (i a)) ⟩
      (a · ( (i a) · (x · (i (i a))) )) · (i a)
        =⟨ ap (λ y → y · (i a)) (! (associative a (i a) (x · (i (i a))))) ⟩
      (( a · (i a)) · (x · (i (i a))) ) · (i a)
        =⟨ ap (λ y → (y · (x · (i (i a))) ) · (i a)) (inv-r a) ⟩
      (e · (x · (i (i a))) ) · (i a) =⟨ ap (λ y → y · (i a)) (unit-l (x · (i (i a)))) ⟩
      (x · (i (i a))) · (i a) =⟨ associative x (i (i a)) (i a) ⟩
      x · ((i (i a)) · (i a)) =⟨ ap (λ y → x · y) (inv-l (i a)) ⟩
      x · e =⟨ unit-r x ⟩
      x =∎)

    module _ (a : Group.U G) where

      {- We will first prove that the conj-map is a homomorphism -}
      conj-map-is-hom : (g₁ g₂ : U) → conj-map a (g₁ · g₂) == ((conj-map a g₁) · (conj-map a g₂))
      conj-map-is-hom g₁ g₂ =
        a · ((g₁ · g₂) · (i a)) =⟨ ap (λ ϕ → a · ϕ) (associative g₁ g₂ (i a)) ⟩
        a · (g₁ · (g₂ · (i a))) =⟨ ap (λ ϕ → a · (g₁ · ϕ)) (! (unit-l ((g₂ · (i a))))) ⟩
        a · (g₁ · ( e · (g₂ · (i a)))) =⟨ ap (λ ϕ → a · (g₁ · (ϕ · (g₂ · (i a))))) (! (inv-l a)) ⟩
        a · (g₁ · (((i a) · a ) · (g₂ · (i a))))
          =⟨ ap (λ ϕ → a · (g₁ · ϕ) ) (associative (i a) a (g₂ · (i a))) ⟩
        a · (g₁ · ((i a) ·(a · (g₂ · (i a)))))
          =⟨ ap (λ ϕ → a · ϕ) (! (associative g₁ ((i a)) ((a · (g₂ · (i a)))))) ⟩
        a · ((g₁ · (i a)) ·(a · (g₂ · (i a))))
          =⟨ ! (associative a ((g₁ · (i a))) ((a · (g₂ · (i a))))) ⟩
        (a · (g₁ · (i a))) ·(a · (g₂ · (i a))) =∎

      conj-hom : GroupHom G G
      conj-hom = group-hom (conj-map a) conj-map-is-hom

      {- Now we want to prove that conj-map is also an isomorphism -}
      conj-hom-g-f : (b : U) → (conj-map (i a) (conj-map a b)) == b
      conj-hom-g-f b =
        conj-map (i a) (conj-map a b)
          =⟨ ap (λ ϕ → conj-map (i a) (conj-map ϕ b)) (! (inv-inv-is-unit a)) ⟩
        conj-map (i a) (conj-map (i (i a)) b) =⟨ funqeq (conj-map-inv (i a)) b ⟩
        b =∎

      conj-hom-is-equiv : is-equiv (conj-map a)
      conj-hom-is-equiv =
        is-eq (conj-map a) (conj-map (i a)) (λ b → funqeq (conj-map-inv a) b) (conj-hom-g-f)

  conj-aut : (a : U) → G ≃ᴳ G
  conj-aut a = conj-hom a , conj-hom-is-equiv a

{- Based on the previous module we can now give an alternative definition of normal subgroups
   that suits are purposes well, namely we define a subgroup to be normal if the lifted conjugation
   automorphims map the subgroup onto itself -}
is-normal' : {G : Group {α}} (H : Subgrp G) → Set (lsucc α)
is-normal' {G} H = (a : Group.U G) → (lift-iso-over-subgrp {G} {G} (ConjAut.conj-aut a) H) == H

{- This should be equivalent to the usual definition of normal subgroups that we defined in the
   group-basics file. For our purposes it is sufficient to show that is-normal' implies is-normal.
   We will do so in the next module -}
module normal-to-normal' {G : Group {α}} {H : Subgrp G} where

  open Group G
  open Subgrp

  private
  {- the following function takes the subgroup H < G and produces for an element (a : G) the
     conjugated subgroup aH(i a), that is, it applies the lifted conjugation automorphism to the
     subgroup. We denote this as φₐ[H] where φₐ : G → G : x ↦ a · x · (i a) -}
    conj-subgr : (a : U) → Subgrp G
    conj-subgr a =  lift-iso-over-subgrp (ConjAut.conj-aut {G} a) H

    {- Here we show that if two groups G and G' are isomorphic, the isomorphism preserves subgroups.
       Basically we prove that map-lift of an isomorphism does exactly what it is supposed to do  -}
    iso-lift-prop-comp : {G' : Group {α}} → (iso : G ≃ᴳ G') → (h : U) → prop H h
                       → prop ((lift-iso-over-subgrp iso) H) ((GroupHom.f (fst iso)) h)
    iso-lift-prop-comp iso h proph = coe (ap (prop H) (! (is-equiv.g-f (snd iso) h))) proph

    {- As a specific instance of the previous lemma, we can show that φₐ[H], the subgroup H lifted
       over the conjugacy automorphism (conj-aut a), contains all the elements of the form
       a · h · (i a) for h in H
    -}
    lift-subgr-conj : (a : U) → (h : U) → prop H h → prop (conj-subgr a) (a · (h · (i a)))
    lift-subgr-conj a h proph = iso-lift-prop-comp {G} (ConjAut.conj-aut {G} a ) h proph

    {- The following are two obvious auxiliary lemma's that will be useful -}
    eq-subgrps-have-eq-props : {N : Subgrp G} → (p : N == H) → (prop N == prop H)
    eq-subgrps-have-eq-props idp = idp

    eq-props-elts : {N : Subgrp G} → (p : prop N == prop H) → (a : U) → (prop N a) → (prop H a)
    eq-props-elts idp a = coe idp

  {- We can now prove that is-normal' implies is-normal. We are given elements (a : G) and (h : H)
     and we want to prove that a · h · (i a) is in H. Using (is-normal' a) we have a proof that
     φₐ[H] == H as subgroups of G, where φₐ : G → G : x ↦ a · x · (ia) is the conjugation map for
     a. Therefore, their props are equal, and from the 'lift-subgr-conj' lemma we can deduce that
     a · h · (i a) is in φₐ[H], hence we can conclude that it is also in H -}
  is-normal'-to-is-normal : is-normal' H → is-normal H
  is-normal'-to-is-normal Hnorm' = λ a h proph → eq-props-elts {conj-subgr a}
    (eq-subgrps-have-eq-props (Hnorm' a)) ((a · (h · (i a)))) (lift-subgr-conj a h proph)


{- Finally, we prove the second goal of the project in two steps -}
{- Firstly, we show that definable subgroups are normal', according to our alternative defition of
   normal subgroups. This follows straight from the machinery that we set up earlier in the file,
   namely the fact that for all group isomorphism φ : G → H we have φ[f G] == f G. In particular,
   we can apply this to the conjugation automorphisms that we are using in our alternative
   definition of is-normal' -}
def-subgroups-are-normal' : (f : (G : Group {α}) → (Subgrp G)) → (G' : Group {α})
                          → (is-normal' (f G'))
def-subgroups-are-normal' f G' =  λ a → lift-aut-retains-subgrp f (ConjAut.conj-aut a)

{- Lastly, using the is-normal-to-is-normal' function that we set up in the previous module we can
   prove our final goal, that all definable subgroups are normal in HoTT -}
def-subgroups-are-normal : (f : (G : Group {α}) → (Subgrp G)) → (G' : Group {α})
                         → (is-normal (f G'))
def-subgroups-are-normal f G' = normal-to-normal'.is-normal'-to-is-normal {G'} {f G'}
                                  (def-subgroups-are-normal' f G')



{- EXAMPLE : CENTER -}

{- We will need the following auxiliary lemma later on -}
prop-dep-prod : {l j : ULevel} {X : Set l} {Y : X → Set j} (ihp : (x : X) → is-prop (Y x))
              → is-prop ((x : X) → Y x)
prop-dep-prod ihp = all-paths-is-prop (λ f g → λ= (λ x → prop-path (ihp x) (f x) (g x)))

{- We show that the center is a definable subgroup, that is, can be uniformly defined as a
   dependent type, depending on the group G -}
center : (G : Group {α}) → Subgrp G
center G = record { prop = λ g → in-center g ; f = in-center-is-prop ; id = unit-in-center
                  ; comp = center-closed-comp ; inv = center-closed-inv }
  where
    open Group G

    {- Here we define the actual map that returns whether an element is in the center or not -}
    in-center : (g : U) → Set α
    in-center g = (h : U) → (h · g) == (g · h)

    {- Next, we show that this map in-center really is a subgroup -}
    in-center-is-prop : {g : U} → is-prop (in-center g)
    in-center-is-prop = prop-dep-prod (λ x → paths-are-props set)

    unit-in-center : in-center e
    unit-in-center = λ h →
      h · e =⟨ unit-r h ⟩
      h =⟨ ! (unit-l h) ⟩
      e · h =∎

    center-closed-comp : {a b : U} → in-center a → in-center b → in-center (a · b)
    center-closed-comp {a} {b} ac bc = λ h →
      h · (a · b) =⟨ ! (associative h a b) ⟩
      (h · a) · b =⟨ ap (λ φ → φ · b) (ac h) ⟩
      (a · h) · b =⟨ associative a h b ⟩
      a · (h · b) =⟨ ap (λ φ → a · φ) (bc h) ⟩
      a · (b · h) =⟨ ! (associative a b h) ⟩
      (a · b) · h =∎

    center-closed-inv : {a : U} → in-center a → in-center (i a)
    center-closed-inv {a} ac = λ h →
      h · (i a) =⟨ ap (λ φ → φ · (i a)) (! (inv-inv-is-unit h)) ⟩
      (i (i h)) · (i a) =⟨ inv-of-comp a (i h)  ⟩
      i ( a · (i h) ) =⟨ ap (λ φ → i φ) (! (ac (i h))) ⟩
      i ( (i h) · a) =⟨ ! (inv-of-comp (i h) a) ⟩
      (i a) · (i (i h)) =⟨ ap (λ φ → (i a) · φ) (inv-inv-is-unit h) ⟩
      (i a) · h =∎

{- Thus, using the main theorem that we proved in this goal, we can show that the center is normal
-}
center-is-normal : {G : Group {α}} → is-normal (center G)
center-is-normal {G} = def-subgroups-are-normal center G
